src/Impl_vm.v
@@ -28,33 +28,23 @@ Fixpoint copland_compile (t:AnnoTerm): CVM unit :=
   | abseq (x,y) sp t1 t2 =>
       (*e <- get_ev ;;
       p <- get_pl ;; *)
-      pr <- split_ev x sp (*e p*) ;;
-      let '(e2,et2) := pr in
-      (*put_ev e1 ;; *)
+      e2 <- split_ev x sp (*e p*) ;;
       copland_compile t1 ;;
       e1r <- get_ev ;;
-      e1rt <- get_evT ;;
       put_ev e2 ;;
-      put_evT et2 ;;
       copland_compile t2 ;;
       e2r <- get_ev ;;
-      e2rt <- get_evT ;;
-      join_seq (Nat.pred y) e1r e1rt e2r e2rt
+      join_seq (Nat.pred y) e1r e2r
   | abpar (x,y) sp t1 t2 =>
     (*e <- get_ev ;;
     p <- get_pl ;; *)
-    pr <- split_ev x sp (*e p*) ;;
-    let '(e2,et2) := pr in
-    (*put_ev e1 ;; *)
+    e2 <- split_ev x sp (*e p*) ;;
     copland_compile t1 ;;
     e1r <- get_ev ;;
-    e1rt <- get_evT ;;
     put_ev e2 ;;
-    put_evT et2 ;;
     copland_compile t2 ;;
     e2r <- get_ev ;;
-    e2rt <- get_evT ;;
-    join_par (Nat.pred y) e1r e1rt e2r e2rt
+    join_par (Nat.pred y) e1r e2r
 
 
     (*
